

B B C C A
→ Note 5

$\lceil \frac{5}{2} \rceil$ 0 conditionally convergent

9. Compute $\left| \frac{5n-2}{2n+1} - \frac{5}{2} \right| = \left| \frac{2(5n-2) - 5(2n+1)}{4n+2} \right| = \left| \frac{9}{4n+2} \right|$

We need $\left| \frac{9}{4n+2} \right| < \varepsilon \Leftrightarrow n > \frac{1}{\varepsilon} \left(\frac{9}{2} - 1 \right)$

(choose $N = \lceil \frac{1}{\varepsilon} (\frac{9}{2} - 1) \rceil$)

Then, for all $\varepsilon > 0$, for all $n \geq N$, we have $\left| \frac{5n-2}{2n+1} - \frac{5}{2} \right| < \varepsilon$.

10. $\lim_{n \rightarrow \infty} \sqrt{n^2 + 9n + 4} - n$

$$= \lim_{n \rightarrow \infty} \frac{(\sqrt{n^2 + 9n + 4} - n)(\sqrt{n^2 + 9n + 4} + n)}{\sqrt{n^2 + 9n + 4} + n}$$

$$= \lim_{n \rightarrow \infty} \frac{n^2 + 9n + 4 - n^2}{\sqrt{n^2 + 9n + 4} + n} = \lim_{n \rightarrow \infty} \frac{9n + 4}{\sqrt{n^2 + 9n + 4} + n} = \lim_{n \rightarrow \infty} \frac{9 + \frac{4}{n}}{\sqrt{1 + \frac{9}{n} + \frac{4}{n^2}} + 1}$$

$$= \frac{9}{\sqrt{1} + 1} = \frac{9}{2}$$

11. $\frac{1}{n(n+3)} = \frac{A}{n} + \frac{B}{n+3} = \frac{A(n+3) + Bn}{n(n+3)}$

$$A(n+3) + Bn = 1 + 0 \cdot n$$

$$(A+B) \cdot n + A \cdot 3 = 0 \cdot n + 1 \Rightarrow A = \frac{1}{3} \quad B = -\frac{1}{3}$$

$$\frac{1}{n(n+3)} = \frac{1}{3} \left(\frac{1}{n} - \frac{1}{n+3} \right)$$

$$S_N = \sum_{n=1}^N \frac{1}{n(n+3)} = \frac{1}{3} \sum_{n=1}^N \left(\frac{1}{n} - \frac{1}{n+3} \right)$$

$$= \frac{1}{3} \left[1 - \frac{1}{4} + \frac{1}{2} - \frac{1}{5} + \frac{1}{3} - \frac{1}{6} + \frac{1}{4} - \frac{1}{7} + \frac{1}{5} - \frac{1}{8} + \dots + \frac{1}{N} - \frac{1}{N+3} \right]$$

$$\therefore S_N = \frac{1}{3} \left(1 + \frac{1}{2} + \frac{1}{3} - \frac{1}{N+1} - \frac{1}{N+2} - \frac{1}{N+3} \right)$$

$$\text{Let } N \rightarrow \infty \quad S_{\infty} = \frac{1}{3} \left(1 + \frac{1}{2} + \frac{1}{3} \right) = \frac{1}{3} \cdot \frac{11}{6} = \frac{11}{18}$$

12. Using ratio test. Let $a_n = \frac{(x-1)^n}{n!}$ then

$$\lim_{n \rightarrow \infty} \left| \frac{a_{n+1}}{a_n} \right| = \lim_{n \rightarrow \infty} \left(\frac{(x-1)^{n+1}}{(n+1)!} \cdot \frac{n!}{(x-1)^n} \right) = \lim_{n \rightarrow \infty} \left(\frac{x-1}{n+1} \right) = 0$$

So the convergence domain is $(-\infty, +\infty)$

$$13. f(x) = \sum_{n=0}^{\infty} \frac{f^{(n)}(0)}{n!} x^n = \sum_{n=0}^{\infty} \frac{(-1)^n}{(2n)!} x^{2n}$$

Note 8

$$f(0) = 1$$

$$f(0) = \cos 0 = 1$$

$$f'(0) = 0$$

$$\text{Let } f(x) = \cos x$$

$$f'(0) = -\sin x = 0$$

$$f''(0) = -1$$

then we have

$$f''(0) = -\cos x = -1$$

$$f'''(0) = 0$$

$$f'''(0) = \sin x = 0$$

So the function is $f(x) = \cos x$

Using ratio test

$$\left| \frac{a_{n+1}}{a_n} \right| = \left| \frac{(-1)^{n+1} x^{2n+2}}{(2n+2)!} \cdot \frac{(2n)!}{(-1)^n x^{2n}} \right| = \left| \frac{x^2}{(2n+2)(2n+1)} \right| \rightarrow 0$$

as $n \rightarrow \infty$

So the radius of convergence is $R = +\infty$.

$$(4) \quad f(x) = \frac{1}{1-x} = \sum_{n=0}^{\infty} \frac{f^{(n)}(0)}{n!} x^n$$

$$f(x) = (1-x)^{-1} \quad f(0) = 1$$

$$f'(x) = (1-x)^{-2} \quad \text{at } x=0 \quad f'(0) = 1$$

$$f''(x) = 2(1-x)^{-3} \quad f''(0) = 2$$

$$f'''(x) = 3!(1-x)^{-4} \quad f'''(0) = 3!$$

⋮

$$f^{(n)}(0) = n!$$

$$f(x) = \sum_{n=0}^{\infty} x^n$$

Consider the radius of convergence $(-1, 1)$

$$f: (-1, 1) \rightarrow \mathbb{R} \quad f(x) = \sum_{n=0}^{\infty} x^n$$